pancake: shared memory update for stack_to_lab proof done

compiler/backend/proofs/stack_to_labProofScript.sml
@@ -596,6 +596,7 @@ val state_rel_def = Define`
     (∀n v. FLOOKUP s.fp_regs n = SOME v ⇒ t.fp_regs n = v) ∧
     t.mem = s.memory ∧
     t.mem_domain = s.mdomain ∧
+    t.shared_mem_domain = s.sh_mdomain ∧
     t.be = s.be ∧
     t.ffi = s.ffi ∧
     t.clock = s.clock ∧
@@ -615,6 +616,7 @@ val state_rel_def = Define`
     (* might need to be cc_save_regs *)
     (!k n. k ∈ s.ffi_save_regs ==> t.cc_regs n k = NONE) /\
     (∀x. x ∈ s.mdomain ⇒ w2n x MOD (dimindex (:'a) DIV 8) = 0) ∧
+    (∀x. x ∈ s.sh_mdomain ⇒ w2n x MOD (dimindex (:'a) DIV 8) = 0) ∧
     s.code_buffer = t.code_buffer ∧
     s.compile = (λc p. t.compile c (MAP prog_to_section p)) ∧
     (t.compile_oracle = λn. let (c,p,_)  = s.compile_oracle n in
@@ -2344,6 +2346,86 @@ Proof
       rfs[MAP_prog_to_section_Section_num]>>
       fs[o_DEF]))>>
   conj_tac >- (
+    rename [`ShMemOp`] >>rpt gen_tac>>strip_tac>>
+    Cases_on ‘op’>>
+    fs[stackSemTheory.evaluate_def,flatten_def]>>
+    fs[word_exp_def,IS_SOME_EXISTS,wordLangTheory.word_op_def]>>
+    gs[case_eq_thms]>>
+    rveq>>fs[]>>
+    gs[sh_mem_op_def,sh_mem_store_def,sh_mem_load_def,
+       sh_mem_store_byte_def,sh_mem_load_byte_def]>>
+    imp_res_tac state_rel_read_reg_FLOOKUP_regs>>
+    pop_assum (assume_tac o GSYM)>>
+    gs[case_eq_thms]>>rveq>>fs[]
+    >>~- ([‘Halt (FFI_outcome _)’],
+          fs[code_installed_def,call_args_def] >>
+          simp[Once labSemTheory.evaluate_def,asm_fetch_def] >>
+          gs[share_mem_op_def,share_mem_load_def,
+             share_mem_store_def,addr_def]>>
+          TRY (qpat_x_assum ‘get_var r _ = _’ assume_tac>>
+               fs[stackSemTheory.dec_clock_def,stackSemTheory.get_var_def]>>
+               drule_then drule state_rel_read_reg_FLOOKUP_regs>>strip_tac>>
+               pop_assum $ assume_tac o GSYM>> fs[])>>
+          rpt (CASE_TAC>>fs[])>>
+          fs[state_rel_def,dec_clock_def,inc_pc_def]>>
+          gs[])>>
+
+    TRY (qexists_tac ‘0’>>qexists_tac ‘t1’>>fs[state_rel_def]>>NO_TAC)>>
+
+    qpat_x_assum ‘call_args (ShMemOp _ _ _) _ _ _ _ _’ mp_tac
+       (* Load *)
+    >>~- ([‘call_args (ShMemOp Load _ _) _ _ _ _ _’],
+         strip_tac>>
+         qexists_tac`0`>>
+                    qexists_tac ‘dec_clock t1
+                    with <| regs := t1.regs⦇r ↦ Word (word_of_bytes F 0w new_bytes)⦈;
+                            io_regs := shift_seq 1 t1.io_regs;
+                            pc:=t1.pc+1; ffi := new_ffi|>’ >>
+         simp[]>>
+         fs[code_installed_def,call_args_def] >>
+         simp[Once labSemTheory.evaluate_def,asm_fetch_def] >>
+         gs[share_mem_op_def,share_mem_load_def,share_mem_store_def,addr_def]>>
+         fs[state_rel_def,stackSemTheory.dec_clock_def,dec_clock_def,inc_pc_def]>>
+         gs[]>>
+         fs[code_installed_def,call_args_def,shift_seq_def] >>
+         fs[FLOOKUP_UPDATE]>>
+         conj_tac >> rpt strip_tac>-
+          (FULL_CASE_TAC>>gs[APPLY_UPDATE_THM])>>
+         metis_tac[])
+  (* Load *)
+    >>~- ([‘call_args (ShMemOp Load8 _ _) _ _ _ _ _’],
+         strip_tac>>
+         qexists_tac`0`>>
+                    qexists_tac ‘dec_clock t1
+                    with <| regs := t1.regs⦇r ↦ Word (word_of_bytes F 0w new_bytes)⦈;
+                            io_regs := shift_seq 1 t1.io_regs;
+                            pc:=t1.pc+1; ffi := new_ffi|>’ >>
+         simp[]>>
+         fs[code_installed_def,call_args_def] >>
+         simp[Once labSemTheory.evaluate_def,asm_fetch_def] >>
+         gs[share_mem_op_def,share_mem_load_def,share_mem_store_def,addr_def]>>
+         fs[state_rel_def,stackSemTheory.dec_clock_def,dec_clock_def,inc_pc_def]>>
+         gs[]>>
+         fs[code_installed_def,call_args_def,shift_seq_def] >>
+         fs[FLOOKUP_UPDATE]>>
+         conj_tac >> rpt strip_tac>-
+          (FULL_CASE_TAC>>gs[APPLY_UPDATE_THM])>>
+         metis_tac[])>>
+    (* Store *)
+    strip_tac>>
+    qexists_tac`0` >>
+    qexists_tac`dec_clock t1 with <| io_regs := shift_seq 1 t1.io_regs;
+                           pc:=t1.pc+1; ffi := new_ffi|>` >>
+    fs[state_rel_def,stackSemTheory.dec_clock_def,dec_clock_def,inc_pc_def]>>
+    fs[code_installed_def,call_args_def] >>
+    gs[Once labSemTheory.evaluate_def,asm_fetch_def] >>
+    gs[share_mem_op_def,share_mem_load_def,share_mem_store_def,addr_def]>>
+    gs[get_var_def]>>
+    last_assum $ qspecl_then [‘a’,‘Word x’] assume_tac>>
+    last_assum $ qspecl_then [‘r’,‘Word w'’] assume_tac>>
+    res_tac>>fs[]>>
+    fs[dec_clock_def,shift_seq_def,inc_pc_def]>>metis_tac[])>>
+  conj_tac >- (
     rename [`CodeBufferWrite`] >>
     rw[stackSemTheory.evaluate_def,flatten_def]>>
     fs[case_eq_thms]>>
@@ -2732,6 +2814,7 @@ val make_init_def = Define `
      ; fp_regs    := FEMPTY (*TODO: is this right? *)
      ; memory  := s.mem
      ; mdomain := s.mem_domain
+     ; sh_mdomain := s.shared_mem_domain
      ; use_stack := F
      ; use_store := F
      ; use_alloc := F
@@ -2884,7 +2967,8 @@ Theorem state_rel_make_init:
     EVERY sec_labels_ok s.code ∧
     (∀k i n. k ∈ save_regs ⇒ s.io_regs n i k = NONE) ∧
     (∀k n. k ∈ save_regs ⇒ s.cc_regs n k = NONE) ∧
-    (∀x. x ∈ s.mem_domain ⇒ w2n x MOD (dimindex (:α) DIV 8) = 0)
+    (∀x. x ∈ s.mem_domain ⇒ w2n x MOD (dimindex (:α) DIV 8) = 0) ∧
+    (∀x. x ∈ s.shared_mem_domain ⇒ w2n x MOD (dimindex (:α) DIV 8) = 0)
 Proof
   fs [state_rel_def,make_init_def,FLOOKUP_regs]
   \\ eq_tac \\ strip_tac \\ fs []
@@ -3068,6 +3152,7 @@ Theorem full_make_init_semantics:
    (∀k i n. k ∈ save_regs ⇒ t.io_regs n i k = NONE) ∧
    (∀k n. k ∈ save_regs ⇒ t.cc_regs n k = NONE) ∧
    (∀x. x ∈ t.mem_domain ⇒ w2n x MOD (dimindex(:'a) DIV 8) = 0) ∧
+   (∀x. x ∈ t.shared_mem_domain ⇒ w2n x MOD (dimindex(:'a) DIV 8) = 0) ∧
    good_code sp code ∧
    (∀n. good_code sp (FST(SND(coracle n)))) ∧
    10 <= sp ∧
@@ -3345,7 +3430,8 @@ val flatten_line_ok_pre = Q.prove(`
   >>
     pop_assum mp_tac>>EVAL_TAC>>
     pop_assum mp_tac>>EVAL_TAC>>
-    fs[]);
+    fs[]>>
+    Cases_on ‘a’>>EVAL_TAC>>rw[]);
 
 Theorem compile_all_enc_ok_pre:
     byte_offset_ok c 0w ∧
